merge_sort.h
@@ -12,56 +12,33 @@ extern size_t buf2_used;
 
 /*@
   axiomatic count_elem_axiom{
-    logic integer count_elem{L}(int elem, int *arr, integer b, integer e) reads arr[b..e-1];
-    axiom empty :
-        \forall int elem, int *arr, integer b, e; b >= e ==> count_elem(elem, arr, b, e) == 0;
-    axiom append_eq : \forall int elem, int *arr, integer b, e;
-        arr[e] == elem ==> count_elem(elem, arr, b, e+1) == count_elem(elem, arr, b, e) + 1;
-    axiom append_neq : \forall int elem, int *arr, integer b, e;
-        arr[e] != elem ==> count_elem(elem, arr, b, e+1) == count_elem(elem, arr, b, e);
+    logic integer count_elem{L}(int elem, int *arr, integer e) reads arr[0..e-1];
+    axiom empty : \forall int elem, int *arr, integer e; e <= 0 ==> count_elem(elem, arr, e) == 0;
+    axiom append_eq : \forall int elem, int *arr, integer e;
+        e >= 0 && arr[e] == elem ==> count_elem(elem, arr, e+1) == count_elem(elem, arr, e) + 1;
+    axiom append_neq : \forall int elem, int *arr, integer e;
+        e >= 0 && arr[e] != elem ==> count_elem(elem, arr, e+1) == count_elem(elem, arr, e);
   }
 
-  predicate permutation{L1, L2}(int *arr1, int *arr2, integer b, integer e) =
-    \forall int v; count_elem{L1}(v, arr1, b, e) == count_elem{L2}(v, arr2, b, e);
+  predicate permutation{L1, L2}(int *arr1, int *arr2, integer e) =
+    \forall int v; count_elem{L1}(v, arr1, e) == count_elem{L2}(v, arr2, e);
 
+  predicate same_array{L1, L2}(int *arr1, int *arr2, integer e) =
+    \forall integer i; 0 <= i < e ==> \at(arr1[i], L1) == \at(arr2[i], L2);
 
-  lemma perm_eq{L1, L2}: \forall int *arr1, int *arr2, integer b, integer e;
-      (\forall integer i; b <= i < e ==> \at(arr1[i], L1) == \at(arr2[i], L2))
-        ==> permutation{L1, L2}(arr1, arr2, b, e);
-
-  predicate unchanged{L1, L2}(int *arr, integer b, integer e) =
-    \forall integer i; b <= i < e ==> \at(arr[i], L1) == \at(arr[i], L2);
-
-  predicate count_unchanged{L1, L2}(int *arr, integer b, integer e) =
-    \forall int elem; count_elem{L1}(elem, arr, b, e) == count_elem{L2}(elem, arr, b, e);
-
-  lemma unchanged_same_count{L1, L2} :
-    \forall int *arr, integer b, e;
-      unchanged{L1, L2}(arr, b, e) ==> count_unchanged{L1, L2}(arr, b, e);
-
+  lemma perm_eq{L1, L2}: \forall int *arr1, int *arr2, integer e;
+        same_array{L1, L2}(arr1, arr2, e) ==> permutation{L1, L2}(arr1, arr2, e);
 
   predicate sorted{L}(int *arr, integer len) =
     \forall integer i, j; 0 <= i <= j < len  ==> arr[i] <= arr[j];
-
-  lemma unchange_sorted{L1, L2}:
-    \forall int *arr, integer len;
-      unchanged{L1, L2}(arr, 0, len) && sorted{L1}(arr, len)
-      ==> sorted{L2}(arr, len);
-
-
-  lemma sorted_append: \forall int *arr, integer len;
-    sorted(arr, len) && arr[len] >= arr[len - 1] ==> sorted(arr, len + 1);
-
-  lemma sorted_all: \forall int *arr, integer len;
-    sorted(arr, len) ==> \forall integer i, j; 0 <= i <= j < len ==> arr[i] <= arr[j];
 */
 
 
 
 /*@
   predicate count_combine(int* a1, integer size1, int* a2, integer size2, int *out) =
-    \forall int v; count_elem(v, a1, 0, size1) + count_elem(v, a2, 0, size2)
-        == count_elem(v, out, 0, size1 + size2);
+    \forall int v; count_elem(v, a1, size1) + count_elem(v, a2, size2)
+        == count_elem(v, out, size1 + size2);
   lemma count_combine_append_1:
     \forall int *a1, *a2, *out, integer size1, size2;
         count_combine(a1, size1, a2, size2, out) && a1[size1] == out[size1 + size2]
@@ -89,15 +66,6 @@ extern size_t buf2_used;
 void merge(int *arr1, size_t len1, int *arr2, size_t len2, int *out);
 
 /*@
-  requires \valid(out + (0 .. len-1));
-  requires \valid_read(in + (0 .. len-1));
-  requires \separated(in + (0 .. len-1), out + (0 .. len-1));
-  assigns out[0..len-1];
-  ensures \forall integer i; 0 <= i < len ==> in[i] == out[i];
-*/
-void arrcpy(int *out, const int *in, size_t len);
-
-/*@
   requires \valid(arr + (0 .. len - 1));
   requires \separated(arr + (0.. len - 1), (buf1 + (buf1_used .. buf1_used + len - 1)));
   requires \separated(arr + (0.. len - 1), (buf2 + (buf2_used .. buf2_used + len * 2- 1)));
@@ -108,7 +76,7 @@ void arrcpy(int *out, const int *in, size_t len);
   assigns buf1_used;
   assigns buf2_used;
   assigns arr[0 .. (len - 1)];
-  ensures permutation{Pre, Post}(arr, arr, 0, len);
+  ensures permutation{Pre, Post}(arr, 0, len);
   ensures sorted(arr, len);
   ensures \at(buf1_used, Post) == \at(buf1_used, Pre);
   ensures \at(buf2_used, Post) == \at(buf2_used, Pre);
